update

theory/Dynamic_Communication_Analysis.thy
@@ -3,7 +3,7 @@ theory Dynamic_Communication_Analysis
 begin
 
 inductive is_send_path :: "trace_pool \<Rightarrow> chan \<Rightarrow> control_path \<Rightarrow> bool" where
-  Intro: "
+  intro: "
     trpl \<pi>y = Some (\<langle>LET xy = SYNC xe in en; env; \<kappa>\<rangle>) \<Longrightarrow>
     env xe = Some (VClosure (Send_Evt xsc xm) enve) \<Longrightarrow>
     enve xsc = Some (VChan c) \<Longrightarrow>
@@ -11,22 +11,21 @@ inductive is_send_path :: "trace_pool \<Rightarrow> chan \<Rightarrow> control_p
   "
 
 inductive is_recv_path :: "trace_pool \<Rightarrow> chan \<Rightarrow> control_path \<Rightarrow> bool" where
-  Intro: "
+  intro: "
     trpl \<pi>y = Some (\<langle>LET xy = SYNC xe in en; env; \<kappa>\<rangle>) \<Longrightarrow>
     env xe = Some (VClosure (Recv_Evt xrc) enve) \<Longrightarrow>
     enve xrc = Some (VChan c) \<Longrightarrow>
     is_recv_path trpl c \<pi>y
   "
 
-
-inductive every_two_dynamic_paths  :: "(control_path \<Rightarrow> bool) \<Rightarrow> (control_path \<Rightarrow> control_path \<Rightarrow> bool) \<Rightarrow> bool" where
-  "
+inductive every_two  :: "('a \<Rightarrow> bool) \<Rightarrow> ('a \<Rightarrow> 'a \<Rightarrow> bool) \<Rightarrow> bool" where
+  intro: "
     (\<forall> \<pi>1 \<pi>2 .
       P \<pi>1 \<longrightarrow>
       P \<pi>2 \<longrightarrow>
       R \<pi>1 \<pi>2
     ) \<Longrightarrow>
-    every_two_dynamic_paths P R
+    every_two P R
   "
 
 inductive ordered :: "'a list \<Rightarrow> 'a list \<Rightarrow> bool" where
@@ -34,25 +33,25 @@ inductive ordered :: "'a list \<Rightarrow> 'a list \<Rightarrow> bool" where
   right: "prefix \<pi>2 \<pi>1 \<Longrightarrow> ordered \<pi>1 \<pi>2"
 
 inductive one_shot :: "trace_pool \<Rightarrow> chan \<Rightarrow> bool" where
-  "
-    every_two_dynamic_paths (is_send_path trpl c) op= \<Longrightarrow> 
+  intro: "
+    every_two (is_send_path trpl c) op= \<Longrightarrow> 
     one_shot trpl c
   "
 
 inductive fan_out :: "trace_pool \<Rightarrow> chan \<Rightarrow> bool" where
-  Intro: "
-    every_two_dynamic_paths (is_send_path trpl c) ordered \<Longrightarrow>
+  intro: "
+    every_two (is_send_path trpl c) ordered \<Longrightarrow>
     fan_out trpl c
   "
   
 inductive fan_in :: "trace_pool \<Rightarrow> chan \<Rightarrow> bool" where
-  Intro: "
-    every_two_dynamic_paths (is_recv_path trpl c) ordered \<Longrightarrow> 
+  intro: "
+    every_two (is_recv_path trpl c) ordered \<Longrightarrow> 
     fan_in trpl c
   "
 
 inductive one_to_one :: "trace_pool \<Rightarrow> chan \<Rightarrow> bool" where
-  Intro: "
+  intro: "
     fan_out trpl c \<Longrightarrow>
     fan_in trpl c \<Longrightarrow> 
     one_to_one trpl c
